parametrized views with the length of the underlying array

Examples.v
@@ -8,32 +8,52 @@ Axiom FunEquality :
   forall A B (f : A -> B) (g : A -> B),
   f = g <-> forall x, f x = g x.
 
+Definition H0' : 0 < 6.
+Proof. apply le_n_S. apply le_0_n. Qed.
+Definition H1' : 1 < 6.
+Proof. repeat apply le_n_S. apply le_0_n. Qed.
+Definition H2' : 2 < 6.
+Proof. auto. Qed.
+Definition H3' : 3 < 6.
+Proof. auto. Qed.
+Definition H4' : 4 < 6.
+Proof. auto. Qed.
+Definition H5' : 5 < 6.
+Proof. auto. Qed.
+
 Example testmap :
   (map reverse (group 3 (identity_view (3*2)))) = 
   (fun x y => match (x,y) with 
-            | (idx _ 0 _,idx _ 0 _) => 2
-            | (idx _ 0 _,idx _ 1 _) => 1
-            | (idx _ 0 _,idx _ 2 _) => 0
-            | (idx _ 1 _,idx _ 0 _) => 5
-            | (idx _ 1 _,idx _ 1 _) => 4
-            | (idx _ 1 _,idx _ 2 _) => 3
-            | _ => 0
+            | (idx _ 0 _,idx _ 0 _) => idx 6 2 H2'
+            | (idx _ 0 _,idx _ 1 _) => idx 6 1 H1'
+            | (idx _ 0 _,idx _ 2 _) => idx 6 0 H0'
+            | (idx _ 1 _,idx _ 0 _) => idx 6 5 H5'
+            | (idx _ 1 _,idx _ 1 _) => idx 6 4 H4'
+            | (idx _ 1 _,idx _ 2 _) => idx 6 3 H3'
+            | _ => idx 6 0 H0'
 end).
 Proof.
   simpl. unfold map. unfold identity_view. unfold group. unfold reverse. 
   apply FunEquality. intros. apply FunEquality. intro y. destruct x as [x Hx]. destruct y as [y Hy]. destruct x.
-  - simpl. destruct y. reflexivity. destruct y. reflexivity. destruct y. reflexivity. exfalso. inversion Hy. inversion H0. inversion H2. inversion H4.
+  - simpl. destruct y. apply unif_Idx. destruct y. apply unif_Idx. destruct y. apply unif_Idx. exfalso. inversion Hy. inversion H0. inversion H2. inversion H4.
   - destruct x.
-    + simpl. destruct y. reflexivity. destruct y. reflexivity. destruct y. reflexivity. exfalso. inversion Hy. inversion H0. inversion H2. inversion H4.
+    + simpl. destruct y. apply unif_Idx. destruct y. apply unif_Idx. destruct y. apply unif_Idx. exfalso. inversion Hy. inversion H0. inversion H2. inversion H4.
     + exfalso. inversion Hx. inversion H0. inversion H2.
 Qed.
 
+Lemma inf : forall s n (i : Idx n),
+  s >= n -> to_nat i < s.
+Proof.
+  intros.
+  apply Nat.le_trans with (m := n).
+  apply BoundedInt. apply H.
+Qed.
 
-Definition identity {T : List nat} {n : nat} (v : ViewArray[[T;n]]) : ViewArray[[;n]] :=
-  fun i => to_nat i.
+Definition index_identity {s : nat} {T : List nat} {n : nat} (H : s >= n) (v : ViewArray s [[T;n]]) : ViewArray s [[;n]] :=
+  fun i => idx s (to_nat i) (inf s n i H).
 
-Example ok :
-  (forall T n, preserve_Injectivity (identity) (A := (n::T))) -> False.
+Example index_identity_does_not_preserve_injectivity :
+  (forall s T n (H : s >= n), preserve_Injectivity (index_identity H) (s := s) (A := (n::T))) -> False.
 Proof.
   intros.
   unfold preserve_Injectivity in H.
@@ -44,7 +64,8 @@ Proof.
     apply preserve_Injectivity_implies_preserving_view_injectivity. apply group_preserves_injectivity.
     apply H2. apply identity_view_injective.
   assert (((idx 2 1 H1,I), (idx 2 0 H0,I)) = ((idx 2 0 H0,I), (idx 2 0 H0,I))).
-  apply H with (v := (group 2 (identity_view (2*2)))) (C := (2::[]))
+  assert ((2*2) >= 2). simpl. auto.
+  apply H with (v := (group 2 (identity_view (2*2)))) (H := H3) (C := (2::[]))
       (i := (idx 2 1 H1,I))
       (x := (idx 2 0 H0,I))
       (j := (idx 2 0 H0,I))
